WIP ***NO_CI***

examples/seplogic/Lang.fst
@@ -3,15 +3,17 @@ module Lang
 open FStar.Seq
 open FStar.Set
 
-assume val size:nat
+type addr = nat
 
-type addr = n:nat{n < size}
-
-type heap = set addr * (s:seq nat{length s = size})
+type heap = {
+  
+  set addr * (s:seq nat{length s = size})
 
 let dom (s:heap) :set addr = fst s
 
 let memory (s:heap) :(s:seq nat{length s = size}) = snd s
+
+let equal (h1:heap) (h2:heap)
 
 let op_String_Access (s:heap) (id:addr) :nat = index (memory s) id
 let op_String_Assignment (s:heap) (id:addr) (v:nat) :heap = (dom s, Seq.upd (memory s) id v)
@@ -20,18 +22,18 @@ let contains (s:heap) (id:addr) :Type0 = Set.mem id (dom s)
 let disjoint (s1:heap) (s2:heap) :Type0 = Set.disjoint (dom s1) (dom s2)
 
 let join (s1:heap) (s2:heap{disjoint s1 s2}) :(s:heap{dom s == Set.union (dom s1) (dom s2)              /\
-                                                         (forall (i:addr). s1 `contains` i ==> s.[i] == s1.[i]) /\
-                                                         (forall (i:addr). s2 `contains` i ==> s.[i] == s2.[i])})
+                                                      (forall (i:addr). s1 `contains` i ==> s.[i] == s1.[i]) /\
+                                                      (forall (i:addr). s2 `contains` i ==> s.[i] == s2.[i])})
   = admit ()
 
 type loop_result (a:Type0) =
-  | Done : v:a -> loop_result a
-  | Again: i:nat -> loop_result a
+  | Done : v:a   -> loop_result a
+  | Again: acc:a -> loop_result a
 
 noeq type command :Type0 -> Type =
   | Return: #a:Type -> v:a -> command a
   | Bind  : #a:Type0 -> #b:Type0 -> c1:command a -> c2:(a -> command b) -> command b
-  | Loop  : #a:Type0 -> i:nat -> f:(nat -> command (loop_result a)) -> command a
+  | Loop  : #a:Type0 -> acc:a -> f:(a -> command (loop_result a)) -> command a
   | Fail  : #a:Type0 -> command a
   | Read  : id:addr -> command nat
   | Write : id:addr -> v:nat -> command unit
@@ -45,28 +47,44 @@ assume val interpreted_in (#a:Type0) (c:command a) (h:heap) :Tot (a * heap)
 
 type heap_predicate = heap -> Type0
 
-let emp :heap_predicate
-  = fun h ->
-    let dom, _ = h in
-    dom == Set.empty
+let emp (h:heap) :Type0 = dom h == Set.empty
 
-let points_to (id:addr) (n:nat) :heap_predicate
-  = fun h ->
-    let dom, m = h in
-    dom == Set.singleton id /\ index m id == n
+let lemma_disjoint_emp (h1:heap) (h2:heap)
+  :Lemma (requires (emp h2))
+         (ensures  (disjoint h1 h2))
+	 [SMTPat (disjoint h1 h2); SMTPat (emp h2)]
+  = assert (Set.equal (Set.intersect (dom h1) (dom h2)) Set.empty)
 
-let lift (phi:Type0) :heap_predicate
-  = fun h -> phi /\ emp h
+let lemma_join_emp (h1:heap) (h2:heap)
+  :Lemma (requires (emp h2))
+         (ensures  (disjoint h1 h2 /\ join h1 h2 == h1))
+  = assert (Set.equal (dom h1) (dom (join h1 h2)));
+    assert (Seq.equal (memory h1) (memory (join h1 h2)))
 
-let exists_x (#a:Type0) (pred:a -> heap_predicate) :heap_predicate
-  = fun h -> exists (x:a). pred x h
+let points_to (id:addr) (n:nat) (h:heap) :Type0 = dom h == Set.singleton id /\ h.[id] == n
 
-let star (p:heap_predicate) (q:heap_predicate) :heap_predicate
-  = fun h -> exists (h1:heap) (h2:heap). disjoint h1 h2 /\ h == join h1 h2 /\ p h1 /\ q h2
+let lift (phi:Type0) (h:heap) :Type0 = phi /\ emp h
+
+let exists_x (#a:Type0) (pred:a -> heap_predicate) (h:heap) :Type0
+  = exists (x:a). pred x h
+
+let star (p:heap_predicate) (q:heap_predicate) (h:heap) :Type0
+  = exists (h1:heap) (h2:heap). disjoint h1 h2 /\ h == join h1 h2 /\ p h1 /\ q h2
 
 let iff (p:heap_predicate) (q:heap_predicate) :Type0 = forall (h:heap). p h <==> q h
 
 let imp (p:heap_predicate) (q:heap_predicate) :Type0 = forall (h:heap). p h ==> q h
+
+(* some algebraic laws on the predicates *)
+
+let lemma1_helper (phi:Type0) (p:heap_predicate) (q:heap_predicate) (h:heap)
+  :Lemma (requires ((phi ==> (p `imp` q)) /\
+                    (star p (lift phi) h)))
+         (ensures  (q h))
+  = assert (exists (h1:heap) (h2:heap). disjoint h1 h2 /\ h == join h1 h2 /\ p h1 /\ ((lift phi) h2) /\ emp h2 /\ phi /\ q h1);
+    admit ()
+
+
 
 type c_pre            = heap_predicate
 type c_post (a:Type0) = a -> heap_predicate
@@ -75,24 +93,62 @@ type hoare_triple (#a:Type0) (pre:c_pre) (c:command a) (post:c_post a)
   = forall (h0:heap) (h1:heap) (r:a). (pre h0 /\ (c `interpreted_in` h0 == (r, h1))) ==> post r h1
 
 (* all the following rules are conditioned on termination *)
-val lemma_return (#a:Type0) (v:a) (c:command a{c == Return v}) (pre:c_pre)
+let lemma_return (#a:Type0) (v:a) (pre:c_pre)
   :Lemma (requires True)  
          (ensures (let post :(c_post a) = fun r -> pre `star` (lift (r == v)) in
-                   hoare_triple pre c post))
+                   hoare_triple pre (Return v) post))
+  = admit ()
 
-val lemma_bind (#a:Type0) (#b:Type0) (c1:command a) (c2:a -> command b) (c:command b{c == Bind c1 c2})
+let lemma_bind (#a:Type0) (#b:Type0) (c1:command a) (c2:a -> command b)
   (pre:c_pre) (post:c_post b)
   :Lemma (requires (exists (q:c_post a). (hoare_triple pre c1 q /\ (forall (r:a). hoare_triple (q r) (c2 r) post))))
-	 (ensures  (hoare_triple pre c post))
+	 (ensures  (hoare_triple pre (Bind c1 c2) post))
+  = admit ()
 
-val lemma_loop (#a:Type0) (i:nat) (f:nat -> command (loop_result a)) (c:command a{c == Loop i f}) (inv:c_post (loop_result a))
-  :Lemma (requires (forall (j:nat). hoare_triple (inv (Again j)) (f j) inv))
-         (ensures  (hoare_triple (inv (Again i)) c (fun r -> inv (Done r))))
+let lemma_loop (#a:Type0) (acc:a) (f:a -> command (loop_result a)) (inv:c_post (loop_result a))
+  :Lemma (requires (forall (j:a). hoare_triple (inv (Again j)) (f j) inv))
+         (ensures  (hoare_triple (inv (Again acc))
+	                         (Loop acc f)
+				 (fun r -> inv (Done r))))
+  = admit ()
 
-val lemma_fail (#a:Type0) (c:command a{c == Fail #a})
+let lemma_fail (#a:Type0)
   :Lemma (requires True)
-         (ensures  (hoare_triple (lift False) c (fun _ -> lift False)))
+         (ensures  (hoare_triple (lift False) (Fail #a) (fun _ -> lift False)))
+  = admit ()
 
-val lemma_consequence (#a:Type0) (c:command a) (p':c_pre) (q':c_post a)
-  :Lemma (requires (forall (p:c_pre) (q:c_post a). hoare_triple p c q /\ p' `imp` p /\ (forall r. q r `imp` q' r)))
+(* making it let ... = admit () does not verify *)
+assume val lemma_consequence (#a:Type0) (c:command a) (p':c_pre) (q':c_post a)
+  :Lemma (requires (forall (p:c_pre) (q:c_post a). hoare_triple p c q /\ p' `imp` p /\ (forall (r:a). q r `imp` q' r)))
          (ensures  (hoare_triple p' c q'))
+
+let lemma_read (id:addr) (r:c_post nat)
+  :Lemma (requires True)
+         (ensures  (hoare_triple (exists_x (fun v -> id `points_to` v `star` (r v)))
+	                         (Read id)
+				 (fun (x:nat) -> (id `points_to` x) `star` (r x))))
+  = admit ()
+
+let lemma_write (id:addr) (v:nat)
+  :Lemma (requires True)
+         (ensures  (hoare_triple (exists_x (fun v' -> id `points_to` v'))
+	                         (Write id v)
+				 (fun _ -> id `points_to` v)))
+  = admit ()
+
+let lemma_alloc (u:unit)
+  :Lemma (requires True)
+         (ensures  (hoare_triple emp Alloc (fun r -> r `points_to` 0)))
+  = admit ()
+
+let lemma_free (id:addr)
+  :Lemma (requires True)
+         (ensures  (hoare_triple (exists_x (fun v -> id `points_to` v))
+	                         (Free id)
+				 (fun _ -> emp)))
+  = admit ()
+
+(* get the nice x <-- c1; c2 syntax *)
+let bind (#a:Type0) (#b:Type0) (c1:command a) (c2:a -> command b) :command b = Bind c1 c2
+
+
